Solved Ex. 3.12.

Reg.thy
@@ -22,7 +22,7 @@ type_synonym reg = nat
 type_synonym rstate = "reg \<Rightarrow> val"
 
 datatype instr =
-  LDI int reg |
+  LDI val reg |
   LD vname reg |
   ADD reg reg
 
@@ -57,6 +57,54 @@ done
 lemma correctness : "exec ( comp a r ) s rs r = aval a s"
   apply ( induction a arbitrary: r s rs )
   apply ( auto simp: append_compose immutable_lesser_states )
+done
+
+
+
+datatype instr0 =
+  LDI0 int |
+  LD0 vname |
+  MV0 reg |
+  ADD0 reg
+
+fun exec01 :: "instr0 \<Rightarrow> state \<Rightarrow> rstate \<Rightarrow> rstate" where
+  "exec01 ( LDI0 i ) s rs = rs ( 0 := i )" |
+  "exec01 ( LD0  x ) s rs = rs ( 0 := ( s x ) )" |
+  "exec01 ( MV0 r ) s rs = rs ( r := ( rs 0 ) )" |
+  "exec01 ( ADD0 r ) s rs = rs ( 0 := ( rs 0 + rs r ) )"
+
+fun exec0 :: "instr0 list \<Rightarrow> state \<Rightarrow> rstate \<Rightarrow> rstate" where
+  "exec0 [] _ rs = rs" |
+  "exec0 ( i # is ) s rs = exec0 is s ( exec01 i s rs )"
+
+
+
+fun comp0 :: "aexp \<Rightarrow> reg \<Rightarrow> instr0 list" where
+  "comp0 ( N i ) r = [ LDI0 i , MV0 r ]" |
+  "comp0 ( V x ) r = [ LD0 x , MV0 r ]" |
+  "comp0 ( Plus a1 a2 ) r = comp0 a1 ( r + 1 ) @  comp0 a2 ( r + 2 )  @
+                            [ LDI0 0 , ADD0 ( r + 1 ) , ADD0 ( r + 2 ) , MV0 r ]"
+
+lemma exec0_append_compose : "exec0 ( is1 @ is2 ) s rs = exec0 is2 s ( exec0 is1 s rs )"
+  apply ( induction is1 arbitrary: rs )
+  apply ( auto )
+done
+
+lemma exec0_immutable_lesser_states :
+  "( r2 > r1 \<and> r1 > 0 ) \<Longrightarrow> exec0 ( comp0 a r2 ) s rs r1 = rs r1"
+
+  apply ( induction a arbitrary: r2 rs )
+  apply ( auto simp: exec0_append_compose )
+done
+
+lemma "exec0 ( comp0 a r ) s rs r = exec0 ( comp0 a r ) s rs 0"
+  apply ( induction a r rule: comp0.induct )
+  apply ( auto simp: exec0_append_compose)
+done
+
+lemma exec0_correctness : "exec0 ( comp0 a r ) s rs r = aval a s"
+  apply ( induction a arbitrary: r s rs )
+  apply ( auto simp: exec0_append_compose exec0_immutable_lesser_states )
 done
 
 end
